\documentclass[%
% handout,
%draft
]{beamer}
\usetheme[shadow]{ComputationalLogic}

\input{PREAMBLE/BPackages.tex}	% \usepackage{mystyle}

\title[Completeness]{Completeness of }
\author[{A$\ell$M}]{%
	Alexander Maringele
}
\institute[UIBK]{%
	{alexander.maringele@gmail.com}
}
% \date{May 9th, 2017}




\begin{document}
\titleframe

\begin{frame}
    \nocite{GK2004csl}
    \bibliographystyle{plain}
    \bibliography{biblio.bib}
\end{frame}


\section{Preliminaries}

\subsection{Clauses, closures and orderings}

\begin{frame}

    \begin{itemize}
        \item a clause $C$ is a multiset of literals
        \item literals are (in)equations of first order terms
        \item a closure $C\cdot\sigma$ is a pair of clause $C$ and substitution $\sigma$
        \item orderings
    \end{itemize}
    \begin{align*}
        &\succG
        \tag*{order on ground terms, literals, and clauses defined by}
        \\
        \tag*{a total, well-founded, and monotone extension of}
        \\
        \tag*{a total simplification ordering $\succG'$ on ground terms}
        \\
        \\
        &\succL
        \tag*{an arbitrary total well-founded extension of $\succG$ such that}
        \\
        && L\sigma\succG L'\sigma' &\Rightarrow L\cdot\sigma\succL L'\cdot\sigma'\tag*{}
        \\
        \\
        &\succC \tag*{an arbitrary total well-founded extension of $\succG$ such that }
        \\
        && C\tau\succG D\rho\text)
        &\Rightarrow C\cdot\tau\succC D\cdot\rho   \tag*{}
        \\
        && (C\tau=D\rho\text{ and }C\theta = D)
        &\Rightarrow C\cdot\tau\succC D\cdot\rho   \tag*{}
    \end{align*}
\end{frame}

\section{Unit Paramodulation}
\begin{frame}{Unit Paramodulation}

    \begin{definition}
    \input{SNIPPETS/UPI}
    where
    \input{SNIPPETS/UPC}
    \end{definition}

    \vspace{0.7em}
    \begin{remark}
    The set of literal closures
    $\{\,
    (\mf(x)\mEQ\mb)\cdot\{x\to\ma\},\, 
    \ma\mEQ \mb,\,
    \mf(\mb)\mNE\mb\,
    \}$ is inconsistent,
    but 
    with $\ma\succG\mb$ 
    the empty clause is not derivable.
    \end{remark}
    
    
\end{frame}



\begin{frame}[allowframebreaks]
    
    \begin{definition}
        
        For a set of literal closures $\mcL$ and 
        arbitrary ground term rewrite system $R$ we define
        \begin{gather*}
            irred_R(\mcL) = \{
                L'\cdot\sigma' \mid
                L'\cdot\sigma'\in\mcL,
                \sigma'\text{ is irreducible w.r.t.~}R
            \}
        \end{gather*}
    
    A literal closure $L\cdot\sigma$ is UP-redundant $\mcL$ if
    \begin{gather*}
    R \cup irred_R(\mcL_{L\cdot\sigma\succL}) \vDash L\sigma
    \end{gather*}
    for any ground term rewrite system $R$ and 
    \begin{gather*}
        \mcL_{L\cdot\sigma\succL} = \{
            L'\cdot\sigma' \mid
            L'\cdot\sigma'\in\mcL,
            L\cdot\sigma\succL L'\cdot\sigma'
        \}
    \end{gather*}

    oriented by $\succG$ where $\sigma$ is irreducible w.r.t.~$R$.
    \vspace{0.7em}

    $\mcR_{UP}$ denotes the set of all UP-redundant closures in $\mcL$.






\end{definition}
\end{frame}

\section{Saturation}
\subsection{Satuaration}
\begin{frame}[allowframebreaks]{Saturation}
    \begin{definition}
        A UP-{ saturation process} is
        a sequence \( \{ \mcL_i \}_{i=0}^\infty \)
        of sets of literal closures where
        \( \mcL_{i+1} \) can be obtained from
        \( \mcL_i \)
        by { adding} a conclusion of an UP-inference with premises in $\mcL_i$
        or by { removing} a UP-redundant w.r.t.~\(\mcL_i\) closure:
        \begin{gather*}
            \mcL_{i+1} = \left\{
                \begin{array}{lclc}
                    \mcL_i \cup\,\emptyclause
                    &\text{if}
                    &
                        \mcL_i\ni(s\mNE t)\cdot\tau,\ {}
                        s\tau = t\tau,\ {}
                        \mu=\mgu(s,t)
                    \\
                    \mcL_i \backslash L\cdot\sigma
                    &\text{if}
                    &R \cup \irred_R(\mcL_{L\cdot\sigma\succL}) \entails L\sigma
                    \\
                    \mcL_i \cup\, L[r]\theta\cdot\rho
                    &\text{if}
                    &\left\{\begin{array}{l}
                        (\ell\mEQ r)\cdot\sigma\in\mcL_i,\ {}
                        L[\ell']\cdot\sigma'\in\mcL_i
                        \\
                        % \mcL_i\ni(l\mEQ r)\cdot\sigma,\ {}
                        \ell\sigma\succG r\sigma,\ {}
                        \theta=\mgu(\ell,\ell'),
                        \\
                        % \mcL_i\ni L[l']\cdot\sigma',\ {}
                        \ell'\notin\mcV,\ {}
                        \ell\sigma = \ell'\sigma' = \ell'\theta\rho,
                    \end{array}\right.
                    \\
                    \mcL_i
                    &&\text{otherwise}
                \end{array}
            \right.
        \end{gather*}
    \end{definition}
    \newpage

    \begin{definition}
        Let \( \mcL^\infty \) be the set of persistent closures,
        i.e.~the lower limit of the sequence.
        The process is { fair} if for every UP-inference
        with premesis in \( \mcL^\infty \) the conclusion is UP-redundant
        w.r.t.~\(\mcL_j\) for some \(j\).

        For a set of literals \( \mcL \) we define
        the saturated set of literal closures
        \( \mcL^{sat} = \mcL^\infty\backslash\mcR_{UP}(\mcL^\infty) \)
        for some UP-saturation process
        \( \{ \mcL_i\}_{i=0}^\infty \)
        with $\mcL_0 = \mcL$.
    \end{definition}

    \begin{lemma}
        The set \( \mcL^{sat} \) is unique because
        for any two UP-fair saturation processes
        \(\{ \mcL_i
            \}_{i=0}^\infty\) and
            \(\{ \mcL'_i
            \}_{i=0}^\infty\)
            with $\mcL_0 = \mcL'_0$ we have
            \begin{gather*}
                \mcL^\infty \backslash \mcR_{UP}(\mcL^\infty)
                =
                \mcL'^\infty \backslash \mcR_{UP}(\mcL'^\infty)
            \end{gather*}
    \end{lemma}
\end{frame}

\subsection{Inst-Redundancy}

% \begin{frame}
%     $\mcR_{Inst}(S)$

%     selection function,

%     S-relevant
% \end{frame}

% \begin{frame}
%     \begin{Lemma}
%         Let $\mcI$ be an arbitrary total consistant extension of $\mcI_S$.

%         Then for every $C\in S$ and $\sigma:\mcV\to\mcTFf$.
%         \begin{align*}
%             \mcI &\models C\cdot\sigma
%         \end{align*}
%     \end{Lemma}

%     \begin{proof}
%         Assume minimal w.r.t.~$\succC$
%         ground instance $D'\cdot\sigma'$ of S with $\mcI\not\models D'\cdot\sigma'$.
%     \end{proof}
% \end{frame}

\subsection{Construction}
\begin{frame}
    Let $\mcL$ be a set of literal closures.
    
    Assume $\mcL\bot$ is satisfiable and
    $\emptyclause\not\in\mcL^{sat}$.

    We define by induction on $\succL$.
    Assume $L = L'\cdot\sigma \in\mcL^{sat}$
    \begin{align*}
        I_L &= \bigcup_{L\succL M}\epsilon_M
        \\
        R_L &= \{ s \to t \mid s\mEQ t\in I_L, s\succG t \}
        \\
        \epsilon_L &= \left\{
            \begin{array}{cl}
                \emptyset &\text{if }
                L'\sigma\text{ reducible by }R_L
                \\
                \emptyset &\text{if }
                I_L\vDash L'\sigma
                \text{ or }
                I_L\vDash \overline{L'}\sigma
                \\
                \{ L'\sigma \}
                &L'\sigma\text{ irreducible by }R_L\text{ and undefined in }I_L
            \end{array}
        \right.\\
        I_S &= \bigcup_{L\in\mcL^{sat}} \epsilon_L
        \qquad\qquad
        R_S = \bigcup_{L\in\mcL^{sat}} R_L
    \end{align*}
\end{frame}



% \subsection{$M\cdot\tau$ is irreducible by $R_S$}
% \begin{frame}[allowframebreaks]{$M\cdot\tau$ is irreducible}
%     % \begin{lemma}
%     %     Let $M\cdot\tau = \min_{\succL}
%     %      \left\{
%     %          M'\cdot\tau' \mid
%     %          M'\cdot\tau' \in irred_{R_S}(\mcL_S^{sat}),
%     %          \mcI \not\models M'\tau'
%     %      \right\}$

%     %     Then, $M\cdot\tau$ is irreducible by $R_S$.
%     % \end{lemma}

%         Let
%             $M\cdot\tau = \min_{\succL}\!
%         \left\{\, 
%             L'\cdot\tau' \mid
%             L'\cdot\sigma' \in irred_{R_S}(\mcL_S^{sat}),\,
%             \mcI \not\models M'\tau'\, 
%         \right\}$
        
%         \textcolor{gray}{(There is at least one $L'\cdot\sigma'\in irred_{R_S}(\mcL_S^{sat})$ false in $\mcI$)}
        
%         \vspace{0.7em}
%         Assume 
%         \begin{itemize}
%             \item $M\cdot\tau$ is reducible by $(\ell\to r)\in R_S$
%             \item $(\ell\to r)$ is produced by $(\ell'\mEQ r')\cdot\rho\in\mcL_S^{sat}$
%         \end{itemize}

%         Bei construction $\tau$ is irreducible by $R_S$.

%         Hence UP-inference is applicable:
%         % and we derive $M[r']\theta\cdot\mu$
%         % from $(\ell'\mEQ r')\cdot\rho$ and $M[\ell'']\cdot\tau$
%         % with $\ell'\rho = \ell''\tau = \ell''\theta\mu$,
%         % $\theta=\mgu(\ell',\ell'')$, and $\mcI\not\models M[r']\theta\mu$
%         \begin{gather*}
%             \infer[UP]
%             {M[r']\theta\cdot\mu}
%             {(\ell'\mEQ r)\cdot\rho & M[\ell'']\cdot\tau}
%             \\
%             \ell'\rho = \ell''\tau = \ell''\theta\mu,\,
%             \theta=\mgu(\ell',\ell''),\,
%             \mcI\not\models M[r']\theta\mu
%         \end{gather*}
%         % % Since both

%         \begin{itemize}
%             \item Assume $M[r']\theta\cdot\mu$ is UP-redundant in $\mcL_S^{sat}$.

%             $\alpha$ is irreducible (lemma ..) by $R_S$. From definiton:
%             % \begin{gather}
%             %     R_S \cup irred_{R_S}(
%             %     \{
%             %         M'\cdot\tau'\mid
%             %         M[r']\theta\cdot\mu \succL M'\tau'
%             %         \} \models M[r']\theta\muu
%             % \end{gather}
%             \item Assume $M[r']\theta\cdot\mu$ is not UP-redundant in $\mcL_S^{sat}$.
%         \end{itemize}
%         % % Since both lead to a contradiction, we must ommit our assumption.
% \end{frame}

%%% FINAL STEP =======================================================================

\subsection{Final step}
\begin{frame}[allowframebreaks]{Final Step}
    \textcolor{gray}{
        $M\cdot\tau = \min_{\succL}\!
        \left\{\, 
            M'\cdot\tau' \mid
            L'\cdot\sigma' \in irred_{R_S}(\mcL_S^{sat}),\,
            \mcI \not\models M'\tau'\, 
        \right\}$}
    \vspace{0.7em}

        We have that $M\cdot\tau$
    \begin{itemize}
        \item is false in $\mcI$
        \item is in $\mcL_S^{sat}$
        \item is irreducible by $R_S$
        \item is not productive.
    \end{itemize}
    \vspace{1em}

    Hence $I_{M\cdot\tau}\models\overline{M}\tau$ 
    with two possible cases:

    \begin{enumerate}
        \item $M\cdot\tau$ is equation $(s\mEQ t)\cdot\tau$  \hfill $I_{M\cdot\tau}\models (s\mNE t)\tau$ 
        \item $M\cdot\tau$ is inequation $(s\mNE t)\cdot\tau$ \hfill $I_{M\cdot\tau}\models (s\mEQ t)\tau$
    \end{enumerate}

\pagebreak
\textcolor{gray}{
    $M\cdot\tau = \min_{\succL}\!
    \left\{\, 
        M'\cdot\tau' \mid
        L'\cdot\sigma' \in irred_{R_S}(\mcL_S^{sat}),\,
        \mcI \not\models M'\tau'\, 
    \right\}$
    \\
    $M\cdot\tau$ is false in $\mcI$, 
    in $\mcL_S^{sat}$, 
    irreducible in $R_S$,
    not productive.}
    \vspace{0.5em}

    \begin{enumerate}
        \item Assume $M\cdot\tau$ is equation $(s\mEQ t)\cdot\tau$:
        \begin{itemize}
            \item $I_{M\cdot\tau}\models (s\mNE t)\tau$
            \item All literals in $I_{M\cdot\tau}$ are irreducible by $R_{M\cdot\tau}$ 
            \item $s\tau$ and $t\tau$ are irreducible by $R_{M\cdot\tau}$
            \item $R_{M\cdot\tau}$ is a convergent term rewrite system
        \end{itemize}
        Hence $(s\mNE t)\tau\in I_{M\cdot\tau}$ and
        produced to $I_{M\cdot\tau}$ by a $(s'\mNE t')\cdot\tau'$.

        Contradicts the minimality of $M\cdot\tau$.
        \vspace{0.5em}
        
        \item Assume $M\cdot\tau$ is inequation $(s\mNE t)\cdot\tau$:
        \begin{itemize}
            \item $I_{M\cdot\tau}\models (s\mEQ t)\tau$
            \item $s\tau$ and $t\tau$ are irreducible by $R_{M\cdot\tau}$
        \end{itemize}
        Hence $s\tau = t\tau$ and equality resolution is applicable.

        Contradicts that the empty clause is not in $\mcL_S^{sat}$.
    \end{enumerate}




       

\end{frame}

\end{document}