% !TeX root = ../mthesis.tex
% !TeX encoding = UTF-8
% !TeX spellcheck = en_US

%\ref{tab:undecidable:PurePredicateLogic}, and
%\ref{tab:undecidable:FunctionsAndEquations}


We look how formulae from these decidable fragments of first order logic 
(Tables \ref{tab:decidedable:FiniteModelProperty} and \ref{tab:decidable:InfinityAxioms})
can be transformed nicely into equisatisfiable set of clauses.
The transformation is easy for formulae where the quantifiers follow a specific pattern where the appearances of the universal quantifier is limited. First we remove leading existential quantifiers and replace their variables with Skolem constants.
Then we remove the trailing existential quantifiers and replace there variables with Skolem functions where the variables of the universal quantifiers are the arguments. After that we remove the remaining universal quantifiers. We transform the remaining formula with constants, functions and a restricted number of free variables into (an equisatisfiable) conjunctive normal form with a suitable procedure. 

\begin{definition}\label{def:prefix:class}
	We describe classes of first order formulae in clausal normal form with triples
	\[
	_{_\CNF}[\, \pi, (p_1,p_2,\ldots), (f_1,f_2,\ldots)\,]_{(=)}
	\]
	where $\pi$ is the maximal number of distinct variables (with multiple occurrences),
	$p_i$ the maximal number of predicates symbols of arity $i$,
	$f_i$ the maximal number of function symbols of arity $i$.
	The equality symbol is not counted as binary predicate symbol.
	Instead the subscript $=$ indicates its presence.
\end{definition}

\begin{table}[hbt]
\begin{align}
\PNF& & \CNF& \tag*{}\\
[\,\exists^{∗}\forall^{∗}, all, (0)&\,]_{=} 
& _{_\CNF}[\,\omega,all, (0)&\,]_{=}
\label{tab:decidable:CNF:1}
\\
[\,\exists^{∗}\forall^2\exists^{∗} , all, (0)&\,] 
& _{_\CNF}[\,2, all, (0,\omega)&\,]
\label{tab:decidable:CNF:2}
\\
[\,all, (\omega), (\omega)&\,]
& _{_\CNF}[\,\omega, (\omega), (\omega)&\,]
\label{tab:decidable:CNF:3}
\\
[\,\exists^{∗}\forall\exists^{∗}, all, all&\,]
& _{_\CNF}[\,1,all, all&\,]
\label{tab:decidable:CNF:4}
\\
[\,\exists^{∗}, all, all&\,]_{=}
& _{_\CNF}[\, 0, all, all&\,]_{=}
\label{tab:decidable:CNF:5}
\\
[\,all, (\omega), (1)&\,]_{=} 
& _{_\CNF}[\,\omega, (\omega), (1)&\,]_{=} 
\label{tab:decidable:CNF:6}
\\
[\,\exists^{∗}\forall\exists^{∗}, all, (1)&\,]_{=}
& _{_\CNF}[\,1, all, (\omega)&\,]_{=}
\label{tab:decidable:CNF:7}
\end{align}
\caption[Transformation]{Transformation into equisatisfiable clausal forms}
\label{tab:decidedable:CNF}
\end{table}

First we substitute existentially quantified leading variables with Skolem constants.

\begin{itemize}
	\item[\ref{tab:decidable:CNF:1}] We get arbitrarily many free variables by dropping the universal quantifiers.
	\item[\ref{tab:decidable:CNF:2}]
	Existentially quantified trailing variables are substituted by binary Skolem functions.
	We get two free variables by dropping the universal quantifiers.
	\item[\ref{tab:decidable:CNF:3}]
	Class is equivalent to $[\,\exists^{∗}\forall^{∗}, (\omega), (\omega)\,]$.
	\item[\ref{tab:decidable:CNF:4}]
	We get one free variables by dropping the universal quantifier.
	\item[\ref{tab:decidable:CNF:5}]
	There are no free variables.
	\item[\ref{tab:decidable:CNF:6}]
	\item[\ref{tab:decidable:CNF:7}]
\end{itemize}

\begin{lemma}\label{lem:unary}
	A formula in $[\,all, (\omega), (\omega)\,]$ is equivalent / equisatisfiable 
	to a formula in $[\,\exists^*\forall^*, (\omega), (\omega)\,]$.
\end{lemma}

\begin{lemma}\label{lem:unary:equals}
	??? A formula in $[\,all, (\omega), (1)\,]_=$ is equivalent / equisatisfiable 
	to a formula in $[\,\exists^*\forall^*, (\omega), (1)\,]_=$ ???
\end{lemma}

\begin{proof} It is sufficient to show for unary predicate and function symbols 
	that $\forall x\exists y\,F\equiv\exists y\forall y\,F$
	where $x,y\in\fvar(F)$. 
	We use induction on the structure of $F$.
	\begin{enumerate}
		\item (base) $F$ is a literal,
		i.e.~a (negated) predicate with one argument term $t$.
		We abbreviate the literal with $L(z)$ if $\var(t) = \{ z \}$. 
		\begin{gather*}
			\forall x \exists y L(x)  \equiv \forall x L(x) \equiv {\colG \exists y} \forall x L(x)
			\qquad\qquad
			\forall x \exists y L(y)  \equiv \exists y L(y) \equiv \exists y{\colG \forall x}  L(y)
		\end{gather*}
		\item (step) $F$ is the negation of a formula.
		\begin{gather*}
		\forall x \exists y\, (\lnot G) 
		\equiv \lnot (\exists x \forall y\, G)
		\defEV[IH] \lnot (\forall y\exists x \, G) 
		\equiv \exists y \forall x\, (\lnot G)
		\end{gather*}
		\item (step) $F$ is the junction $\landlor\in\{\land,\lor\}$ of a “free” literal and a formula.
		\begin{gather*}
		\forall x\exists y\,( L(z) \landlor G) 
		\equiv L(z) \landlor \forall x\exists y\, G
		\defEV[IH]L(z) \landlor \exists y\forall x\, G
		\equiv\exists y\forall x\,( L(z) \landlor G )
		\end{gather*}
		\item (step) $F$ is the conjunction of a “universal” literal and a formula.
		\begin{align*}
		\forall x \exists y\,({L(x)\land G}) 
		&\equiv \forall x\,({L(x)} \land \exists y\,G)
		\equiv \forall x\,L(x)\land \forall x\exists y\,G
		\\&\defEV[IH] \forall x\,{L(x)} \land \exists y\forall x\,G
%		\equiv \exists y\forall x\,({L(x)\land G})
		\equiv\exists y \forall x\,({L(x)\land G})
		\end{align*}
		\item (step) $F$ is the disjunction of an “existential” literal and a formula.
		\begin{align*}
		\forall y \exists x\,({L(x)\lor H}) 
		&\equiv\lnot(\exists y \forall x (L^c(x)\land\lnot H)))\\
		&\defEV[3.]\lnot(\forall x\exists y  (L^c(x)\land\lnot H))) 
		\equiv \exists x\forall y\, (L(x) \land H)
		\end{align*}
		\item (step) $F$ is the conjunction of an “existential” literal and a formula.
		\begin{align*}
		\forall x \exists y\,({L(y)\land H}) 
		&\equiv\lnot(\exists x\forall y \,({L^c(y) \lor \lnot H})) \\
		&\defEV[4.]\lnot(\forall x\exists y \,({L^c(y) \lor \lnot H}) )
		\equiv \exists x\forall y\,(L(y)\land H)
		\end{align*}
		\item (step) $F$ is the disjunction of a “universal” literal and a formula.
		\begin{align*}
		\forall x \exists y\,(L(x)\lor H) 
		&\equiv \lnot (\exists x\forall y\,(L^c(x) \land H)) \\
		&\defEV[4.]\lnot (\forall y\exists x\,(L^c(x) \land\lnot H)) 
		\equiv \exists y \exists x\,(L(x)\lor H))\\
		\end{align*}
	\end{enumerate}
\end{proof}

\begin{proof}
	\begin{enumerate}
		\item $\forall x \exists y\, x\mEQ y$
		\item $\forall x \exists y\, y\mEQ x$
	\end{enumerate}
		
\end{proof}


%% ADDITIONAL MATERIAL %%%%

\begin{table}[hbt]
	\begin{align*}
	[\,\forall\exists\forall, (\omega, 1), (0)&\,] \tag{Kahr 1962}
	\\
	[\,\forall^3 \exists, (\omega, 1), (0)&\,] \tag{Surányi 1959}
	\\
	[\,\forall^{∗} \exists, (0, 1), (0)&\,] \tag{Kalmár-Surányi 1950}
	\\
	[\,\forall\exists\forall^{∗} , (0, 1), (0)&\,]  \tag{Denton 1960}
	\\
	[\,\forall\exists\forall\exists^{∗}, (0, 1), (0)&\,] \tag{Gurevich 1966}
	\\
	[\,\forall^3 \exists^{∗} , (0, 1), (0)&\,] \tag{Kalmár-Surányi 1947}
	\\
	[\,\forall\exists^{∗} \forall, (0, 1), (0)&\,] \tag{Kostyrko-Genenz 1964}
	\\
	[\,\exists^{∗} \forall\exists\forall, (0, 1), (0)&\,] \tag{Surányi 1959}
	\\
	[\,\exists^{∗} \forall^3 \exists, (0, 1), (0)&\,] \tag{Surányi 1959}
	\end{align*}
	\caption{Undecidable prefix classes in pure predicate logic}
	\label{tab:undecidable:PurePredicateLogic}
\end{table}

\begin{table}[hbt]
	\begin{align*}
	[\,\forall, (0), (2)&\,]_{=} \tag{Gurevich 1976}
	\\
	[\,\forall, (0), (0, 1)&\,]_{=} \tag{Gurevich 1976}
	\\
	[\,\forall^2 , (0, 1), (1)&\,] \tag{Gurevich 1969}
	\\
	[\,\forall^2 , (1), (0, 1)&\,] \tag{Gurevich 1969}
	\\
	[\,\forall^2\exists, (\omega, 1), (0)&\,]_{=} \tag{Goldfarb 1984}
	\\
	[\,\exists^{∗}\forall^2\exists, (0, 1), (0)&\,]_{=} \tag{Goldfarb 1984}
	\\
	[\,\forall^2\exists^{∗}, (0, 1), (0)&\,]_{=} \tag{Goldfarb 1984}
	\end{align*}
	\caption{Undecidable prefix classes with functions or equality}
	\label{tab:undecidable:FunctionsAndEquations}
\end{table}


\begin{table}[hbt]
	\begin{gather*}
		\begin{array}{rcccl}
		\text{undecidable} &&\multicolumn{1}{c}{decidable}  & &  \text{classification}
		\\ \\{}
[\,\Pi_?, (p_1, {\colLo 1}), (0)\,] &\supsetneq&
[\,\Pi_?, (p_1, {\colHi 0}), (0)\,]&\subseteq&
[\,all,(\omega),(\omega)\,]
\\[0.5em]		
		\\ \\{}
		[\,\forall\exists\forall, (\omega, 1), (0)\,] &\multirow{9}{*}{$\supsetneq$}&
		\multirow{9}{*}{$[\,\Pi, (p_1, {\colHi 0}), (0)\,]$} &\multirow{9}{*}{$\subseteq$}&
		\multirow{9}{*}{$[\,all,(\omega),(\omega)\,]$}
	\\{}
	[\,\forall^3 \exists, (\omega, 1), (0)\,] &&
	&&
	\\{}
	[\,\forall^{∗} \exists, (0, 1), (0)\,] &&
	&&
	\\{}
	[\,\forall\exists\forall^{∗} , (0, 1), (0)\,]&&
	&&
	\\{}
	[\,\forall\exists\forall\exists^{∗}, (0, 1), (0)\,]&&
	&&
	\\{}
	[\,\forall^3 \exists^{∗} , (0, 1), (0)\,] &&
	&&
	\\{}
	[\,\forall\exists^{∗} \forall, (0, 1), (0)\,] &&
	&&
	\\{}
	[\,\exists^{∗} \forall\exists\forall, (0, 1), (0)\,]&&
	&&
	\\{}
	[\,\exists^{∗} \forall^3 \exists, (0, 1), (0)\,] &&
	&&
\\{}
\\[0.5em]
	[\,\forall, (0), ({\colLo 2})\,]_{=} &\supsetneq&
	[\,\forall, (0), ({\colHi 1})\,]_{=} &\subseteq&[\,all, (\omega), (1)\,]_{=}
	\\{}
	[\,\forall, (0), (0, {\colLo 1})\,]_{=} &\supsetneq&
	[\,\forall, (0), (0, {\colHi 0})\,]_{=}	&\subseteq&[\,all, (\omega), (1)\,]_{=}
	\\[0.5em]
	[\,\forall^2 , (0, {\colN 1}), ({\colLo 1})\,]_{\color{white}=} &\supsetneq&
	[\,\forall^2 , (0, {\colN 1}), ({\colHi 0})\,]_{\color{white}=} &\subseteq&[\,\exists^{∗}\forall^2\exists^{∗} , all, (0)\,]_{\color{white}=}
	\\{}
	%
	{[\,\forall^2 , ({\colN 1}), (0, {\colLo 1})\,]_{\color{white}=}}&\supsetneq&
	[\,\forall^2 , ({\colN 1}), (0, {\colHi 0})\,]_{\color{white}=}&\subseteq&[\,\exists^{∗}\forall^2\exists^{∗} , all, (0)\,]_{\color{white}=}
	\\[0.5em]
	[\,\forall^2\exists, (\omega, {\colLo 1}), (0)\,]_{=} &\subseteq&
	[\,\forall^2\exists, (\omega, {\colHi 0}), (0)\,]_{=} &\subseteq&[\,all, (\omega), (1)\,]_{=}
	\\{}
	%
	[\,\exists^{∗}\forall^2\exists, (0, {\colLo 1}), (0)\,]_{=}&\supsetneq&
		[\,\exists^{∗}\forall^2\exists, (0, {\colHi 0}), (0)\,]_{=}&\subseteq&[\,all, (\omega), (1)\,]_{=}
	\\{}
	[\,\forall^2\exists^{∗}, (0, {\colLo 1}), (0)\,]_{=}&\supsetneq&
	[\,\forall^2\exists^{∗}, (0, {\colHi 0}), (0)\,]_{=}&\subseteq& [\,all, (\omega), (1)\,]_{=}
	\end{array}
	\end{gather*}
\end{table}


