% !TeX root = ../mythesis.tex
% !TeX encoding = UTF-8
% !TeX spellcheck = en_US

\begin{definition}[\cite{Huth:2004:LCS:975331}]\label{def:natural:deduction}
	We recall the rules of \coloremph{natural deduction} for connectives
	equality, and quantifiers in
	Tables~\ref{tab:natural:deduction:connectives},
	\ref{tab:natural:deduction:equality}, and
	\ref{tab:natural:deduction:quantifiers}.
	Natural deduction provides a logical calculus,
	i.e.~a formal proof system for first order logic.
	In these rules
	\( F \) and \( G \) are arbitrary first order sentences,
	the bound variable \( x \) in any quantified formula
	\( \forall x F' \) occurs free in \( F' \),
	first order terms \( s \) and \( t \) are ground,
	and \( \mc \) is a \emph{fresh} constant function symbol,
	i.e.~it did not occur in any formula so far.

\begin{table}[hbt]
\begin{gather*}
\begin{array}{ccccc}
\infer[(\land i)]{F\land G}{F & G}
&
\infer[(\land e_1)]{G}{F \land G}
&
\infer[(\land e_2)]{F}{F \land G}
&
\infer[(\lnot\lnot i)]{\lnot\lnot F}{F}
&
\infer[(\lnot\lnot e)]{F}{\lnot\lnot F}
\\[0.7em]
\infer[(\bot e)]{F}{\bot}
&
\infer[(\lnot e)]{\bot}{F & \lnot F}
&
\infer[\text{LEM}]{F\lor\lnot F}{}
&
\infer[(\lor i_1)]{F\lor G}{F}
&
\infer[(\lor i_2)]{F\lor G}{G}
\\[0.7em]
\infer[(\lnot i)]{\lnot F}{
	\boxed{\begin{array}{c}F \\ \vdots \\ \bot \end{array}}}
&
\infer[\text{PBC}]{F}{
	\boxed{\begin{array}{c}\lnot F \\ \vdots \\ \bot \end{array}}}
&
\infer[({\limp} i)]{F\limp G}{
	\boxed{\begin{array}{c}F \\ \vdots \\ G \end{array}
}}
&
\multicolumn{2}{l}{
	\infer[(\lor e)]{H}{
		F\lor G &
		\boxed{\begin{array}{c}F \\ \vdots \\ H \end{array}} &
		\boxed{\begin{array}{c}G \\ \vdots \\ H \end{array}}
	}
}
\\[0.7em]
&
\multicolumn{3}{r}{
\infer[\text{modus}\atop\text{ponens}]{G}{F & F\limp G}
\qquad
\infer[\text{modus}\atop\text{tollens}]{\lnot F}{F\limp G & \lnot G}
}
&
\end{array}
\end{gather*}
\caption{Natural Deduction Rules for Connectives}\label{tab:natural:deduction:connectives}
\end{table}

\begin{table}[hbt]
	\begin{gather*}
	\infer[({=}e)]{F'\{x\mapsto t\}}{s=t & F'\{x\mapsto s\}}
	\qquad
	\infer[({=}i)]{t=t}{}
	\end{gather*}
	\caption{Natural Deduction Rules for Equality}\label{tab:natural:deduction:equality}
\end{table}

\begin{table}[hbt]
	\begin{gather*}
	\begin{array}{ccc}
	\infer[(\forall e)]{F'\{x\to t\}}{
		\forall x F'
	}
	&&
		\infer[(\exists i)]{\exists x F'}{
		F'\{x\mapsto t \}
	}
	\\[1em]
	\infer[(\forall i)]{\forall x F'}{
		\boxed{
			\begin{array}{cc}
				\mc
				\\
				&\vdots
				\\
				&F' \{x\mapsto \mc\}
			\end{array}} % end of boxed
	}
	&&
	\infer[(\exists e)]{H}{
		\exists x F' &
		\boxed{
			\begin{array}{cc}
				\mc&F' \{ x\mapsto \mc \}
				\\
				&\vdots
				\\
				&H
			\end{array}} % end of boxed
	}
	\end{array}
	\end{gather*}
	\caption{Natural Deduction Rules for Quantifiers}\label{tab:natural:deduction:quantifiers}
\end{table}
\end{definition}